coq/ZF/Meta/Test/Axiom/Foundation.v
@@ -13,12 +13,12 @@ Import ListNotations.
 Definition empty : Decl :=
   {| para := [];
      res  := TySet;
-     body := None |}.
+     body := HoleT TySet |}.
 
 Definition inter : Decl :=
   {| para := [TySet; TySet];
      res  := TySet;
-     body := None |}.
+     body := HoleT TySet |}.
 
 Definition env : Env := Env.fromListT
   [ ("empty"%string, empty)
